a sketch implementation of unification.

theories/Poly/PolyPHOAS.v
@@ -1,10 +1,11 @@
+Require Import ExtLib.Data.HList.
 (** * The proposed meta-theory **)
 
 (*
 (kinds)        k := k -> k | *
 (large types)  l := forall x : k , l | [s]
 (small types)  s := s -> s | s s | x | [b]
-(expr)         e := \ x : s. e | e e | x | e s | [b]
+(expr)         e := \ x : s. e | e e | x | e s | ?u | [b]
 *)
 
 Set Printing Universes.
@@ -17,7 +18,7 @@ Constraint U0 < U1.
 
 (* kinds of small types *)
 Inductive kind : Set :=
-| kStar 
+| kStar
 | kArr (_ _ : kind).
 
 
@@ -30,7 +31,7 @@ Fixpoint kindD (k : kind) : Type@{U1} :=
 (* kinds of large types *)
 Inductive lkind : Set :=
 | lkStar
-| lkArr (_ : kind) (_ : lkind)            
+| lkArr (_ : kind) (_ : lkind)
 | lkArrl (_ _ : lkind)
 .
 
@@ -49,62 +50,81 @@ Fixpoint lkindD (k : lkind) : Type@{U2} :=
 
 (** * Types **)
 (* Small Types *)
-Inductive type (F : kind -> Type) : kind -> Type :=
-| smVar : forall k, F k -> type F k
-| smArr : type F kStar -> type F kStar -> type F kStar
-| smAbs : forall k1 k2, (F k1 -> type F k2) -> type F (kArr k1 k2)
-| smApp : forall k1 k2, type F (kArr k1 k2) -> type F k1 -> type F k2
+Inductive type (Fu : list kind -> kind -> Type@{U1}) (F : kind -> Type@{U1}) : kind -> Type :=
+| smVar : forall k, F k -> type Fu F k
+| smUVar : forall ks k, Fu ks k -> hlist (type Fu F) ks -> type Fu F k
+| smArr : type Fu F kStar -> type Fu F kStar -> type Fu F kStar
+| smAbs : forall k1 k2, (F k1 -> type Fu F k2) -> type Fu F (kArr k1 k2)
+| smApp : forall k1 k2, type Fu F (kArr k1 k2) -> type Fu F k1 -> type Fu F k2
 .
 
-Arguments smVar {_ _} _.
-Arguments smArr {_} _ _.
-Arguments smAbs {_ _ _} _.
-Arguments smApp {_ _ _} _ _.
+Arguments smVar {_ _ _} _.
+Arguments smUVar {_ _ _ _} _ _.
+Arguments smArr {_ _} _ _.
+Arguments smAbs {_ _ _ _} _.
+Arguments smApp {_ _ _ _} _ _.
 
 
 (* Large Types *)
-Inductive ltype (lF : lkind -> Type) (F : kind -> Type) : lkind -> Type :=
-| tsmVar  : forall k, F k -> ltype lF F (lkLift k)
-| tVar  : forall k, lF k -> ltype lF F k
-| tArr : ltype lF F lkStar -> ltype lF F lkStar -> ltype lF F lkStar
-| tPi : forall k, (type F k -> ltype lF F lkStar) -> ltype lF F lkStar
+Inductive ltype (lF : lkind -> Type@{U2}) (Fu : list kind -> kind -> Type@{U1}) (F : kind -> Type@{U1}) : lkind -> Type :=
+| tsmVar  : forall k, F k -> ltype lF Fu F (lkLift k)
+| tsmUVar  : forall ks k, Fu ks k -> hlist (fun x => type Fu F x) ks -> ltype lF Fu F (lkLift k)
+| tVar  : forall k, lF k -> ltype lF Fu F k
+| tArr : ltype lF Fu F lkStar -> ltype lF Fu F lkStar -> ltype lF Fu F lkStar
+| tPi : forall k, (type Fu F k -> ltype lF Fu F lkStar) -> ltype lF Fu F lkStar
 
 (* small type abstraction/application *)
-| tAbs : forall k1 k2, (F k1 -> ltype lF F k2) -> ltype lF F (lkArr k1 k2)
-| tApp : forall k1 k2, ltype lF F (lkArr k1 k2) -> type F k1 -> ltype lF F k2
+| tAbs : forall k1 k2, (F k1 -> ltype lF Fu F k2) -> ltype lF Fu F (lkArr k1 k2)
+| tApp : forall k1 k2, ltype lF Fu F (lkArr k1 k2) -> type Fu F k1 -> ltype lF Fu F k2
 
 (* large type abstraction/application *)
-| tAbsl : forall k1 k2, (lF k1 -> ltype lF F k2) -> ltype lF F (lkArrl k1 k2)
-| tAppl : forall k1 k2, ltype lF F (lkArrl k1 k2) -> ltype lF F k1 -> ltype lF F k2
+| tAbsl : forall k1 k2, (lF k1 -> ltype lF Fu F k2) -> ltype lF Fu F (lkArrl k1 k2)
+| tAppl : forall k1 k2, ltype lF Fu F (lkArrl k1 k2) -> ltype lF Fu F k1 -> ltype lF Fu F k2
 .
 
-Arguments tsmVar {_ _ _} _.
-Arguments tVar {_ _ _} _.
-Arguments tArr {_ _} _ _.
-Arguments tPi {_ _ _} _.
-Arguments tAbs {_ _ _ _} _.
-Arguments tApp {_ _ _ _} _ _.
-Arguments tAbsl {_ _ _ _} _.
-Arguments tAppl {_ _ _ _} _ _.
+Arguments tsmVar {_ _ _ _} _.
+Arguments tsmUVar {_ _ _ _ _} _ _.
+Arguments tVar {_ _ _ _} _.
+Arguments tArr {_ _ _} _ _.
+Arguments tPi {_ _ _ _} _.
+Arguments tAbs {_ _ _ _ _} _.
+Arguments tApp {_ _ _ _ _} _ _.
+Arguments tAbsl {_ _ _ _ _} _.
+Arguments tAppl {_ _ _ _ _} _ _.
 
-Fixpoint liftT {lF F k} (t : type F k) : ltype lF F (lkLift k) :=
-  match t in type _ k return ltype lF F (lkLift k) with
-      smVar x => tsmVar x
-    | smArr t1 t2 => tArr (liftT t1) (liftT t2)
-    | smAbs f => tAbs (fun x => liftT (f x))
-    | smApp f x => tApp (liftT f) x
-  end
-.
+Fixpoint liftT {lF Fu F k} (t : type Fu F k) : ltype lF Fu F (lkLift k) :=
+  match t in type _ _ k return ltype lF Fu F (lkLift k) with
+    smVar x => tsmVar x
+  | smUVar u xs => tsmUVar u xs
+  | smArr t1 t2 => tArr (liftT t1) (liftT t2)
+  | smAbs f => tAbs (fun x => liftT (f x))
+  | smApp f x => tApp (liftT f) x
+  end.
 
-Example idType {lF F} : ltype lF F lkStar :=
-tPi (fun t => liftT (smArr t t)).
+Example idType {lF Fu F} : ltype lF Fu F lkStar :=
+  tPi (fun t => liftT (smArr t t)).
 
-Fixpoint typeD {k} (t : type kindD k) : kindD k :=
+Fixpoint build_Karrow (ls : list kind) (k : kind) : kind :=
+  match ls with
+  | nil => k
+  | cons l ls => kArr l (build_Karrow ls k)
+  end.
+
+Definition kindDu (ls : list kind) (k : kind) : Type :=
+  kindD (build_Karrow ls k).
+
+Fixpoint typeD {k} (t : type kindDu kindD k) : kindD k :=
   match t with
-    | smVar x     => x
-    | smArr t1 t2 => typeD t1 -> typeD t2                                           
-    | smAbs f     => fun x => typeD (f x)
-    | smApp f x   => typeD f (typeD x)
+  | smVar x     => x
+  | @smUVar _ _ ks k u xs =>
+    (fix rec ls xs : (kindDu ls k) -> kindD k :=
+       match xs in hlist _ ls return kindDu ls k -> kindD k with
+       | Hnil => fun x => x
+       | Hcons x xs => fun u => rec _ xs (u (typeD x))
+       end) ks xs u
+  | smArr t1 t2 => typeD t1 -> typeD t2
+  | smAbs f     => fun x => typeD (f x)
+  | smApp f x   => typeD f (typeD x)
   end.
 
 Definition liftType : Type@{U0} -> Type@{U1} := fun x => x.
@@ -115,63 +135,98 @@ Fixpoint lkLiftD (k : kind) : kindD k -> lkindD (lkLift k) :=
     | kArr a b => fun f x => lkLiftD b (f x)
   end.
 
-Fixpoint ltypeD {k} (t : ltype lkindD kindD k) : lkindD k :=
-  match t in ltype _ _ k return lkindD k with
+Fixpoint ltypeD {k} (t : ltype lkindD kindDu kindD k) : lkindD k :=
+  match t in ltype _ _ _ k return lkindD k with
     | tsmVar x => lkLiftD _ x
+    | @tsmUVar _ _ _ ks k u xs =>
+      lkLiftD _ ((fix rec ls (xs : hlist (fun x => type kindDu kindD x) ls) :=
+                    match xs in hlist _ ls
+                          return kindDu ls k -> kindD k
+                    with
+                    | Hnil => fun x => x
+                    | Hcons x xs => fun f => rec _ xs (f (typeD x))
+                    end) ks xs u)
     | tVar x => x
     | tPi f => forall a, ltypeD (f a)
-    | tArr t1 t2 => ltypeD t1 -> ltypeD t2                                           
+    | tArr t1 t2 => ltypeD t1 -> ltypeD t2
     | tAbs f => fun x => ltypeD (f x)
     | tApp f x => ltypeD f (typeD x)
     | tAbsl f => fun x => ltypeD (f x)
     | tAppl f x => ltypeD f (ltypeD x)
   end.
 
+
 (** * Expressions **)
 
 (* Expressions have large types *)
 Inductive expr
-          (lF : lkind -> Type)
-          (F : kind -> Type)
-          (Fe : ltype lF F lkStar -> Type) :
-  ltype lF F lkStar -> Type :=
-| eVar  : forall t, Fe t -> expr lF F Fe t
-| eAbs  : forall (t1 t2 : ltype lF F lkStar), (Fe t1 -> expr lF F Fe t2) -> expr lF F Fe (tArr t1 t2)
-| eApp  : forall (t1 t2 : ltype lF F lkStar), expr lF F Fe (tArr t1 t2) -> expr lF F Fe t1 -> expr lF F Fe t2
-| eTAbs : forall k (tf : type F k -> ltype lF F lkStar), (forall t, expr lF F Fe (tf t)) -> expr lF F Fe (tPi tf)
-| eTApp : forall k (tf : type F k -> ltype lF F lkStar), expr lF F Fe (tPi tf) -> forall t, expr lF F Fe (tf t)
+          (lF : lkind -> Type@{U2})
+          (Ku : list kind -> kind -> Type@{U1})
+          (F : kind -> Type@{U1})
+          (Fu : list (ltype lF Ku F lkStar) -> ltype lF Ku F lkStar -> Type)
+          (Fe : ltype lF Ku F lkStar -> Type) :
+  ltype lF Ku F lkStar -> Type :=
+| eVar  : forall t, Fe t -> expr lF Ku F Fu Fe t
+| eUVar : forall ts t, Fu ts t -> hlist (expr lF Ku F Fu Fe) ts -> expr lF Ku F Fu Fe t
+
+| eAbs  : forall (t1 t2 : ltype lF Ku F lkStar),
+    (Fe t1 -> expr lF Ku F Fu Fe t2) -> expr lF Ku F Fu Fe (tArr t1 t2)
+| eApp  : forall (t1 t2 : ltype lF Ku F lkStar), expr lF Ku F Fu Fe (tArr t1 t2) -> expr lF Ku F Fu Fe t1 -> expr lF Ku F Fu Fe t2
+| eTAbs : forall k (tf : type Ku F k -> ltype lF Ku F lkStar), (forall t, expr lF Ku F Fu Fe (tf t)) -> expr lF Ku F Fu Fe (tPi tf)
+| eTApp : forall k (tf : type Ku F k -> ltype lF Ku F lkStar), expr lF Ku F Fu Fe (tPi tf) -> forall t, expr lF Ku F Fu Fe (tf t)
 .
 
-Arguments eVar  {_ _ _ _} _.
-Arguments eAbs  {_ _ _ _ _} _.
-Arguments eApp  {_ _ _ _ _} _ _.
-Arguments eTAbs {_ _ _ _ _} _.
-Arguments eTApp {_ _ _ _ _} _ _.
+Arguments eVar  {_ _ _ _ _ _} _.
+Arguments eUVar  {_ _ _ _ _ _ _} _ _.
+Arguments eAbs  {_ _ _ _ _ _ _} _.
+Arguments eApp  {_ _ _ _ _ _ _} _ _.
+Arguments eTAbs {_ _ _ _ _ _ _} _.
+Arguments eTApp {_ _ _ _ _ _ _} _ _.
 
-Fixpoint exprD {t : ltype lkindD kindD lkStar} (e : expr lkindD kindD ltypeD t) : ltypeD t :=
-  match e in expr _ _ _ t return ltypeD t with
-    | eVar x => x 
+Section here.
+  Context {lF : lkind -> Type} {Ku : list kind -> kind -> Type} {F : kind -> Type}.
+  Fixpoint build_arrow (ls : list (ltype lF Ku F lkStar)) (rt : ltype lF Ku F lkStar)
+  : ltype lF Ku F lkStar :=
+    match ls with
+    | nil => rt
+    | cons l ls => tArr l (build_arrow ls rt)
+    end.
+End here.
+
+Definition uvarD a b := ltypeD (build_arrow a b).
+
+
+Fixpoint exprD {t : ltype lkindD kindDu kindD lkStar}
+         (e : expr lkindD kindDu kindD uvarD ltypeD t)
+: ltypeD t :=
+  match e in expr _ _ _ _ _ t return ltypeD t with
+    | eVar x => x
+    | @eUVar _ _ _ _ _ ts t u xs =>
+      (fix rec ts
+          (es : hlist (fun t => expr lkindD kindDu kindD uvarD ltypeD t) ts) :
+         (ltypeD (build_arrow ts t)) -> ltypeD t :=
+         match es in hlist _ ts
+               return (ltypeD (build_arrow ts t)) -> ltypeD t
+         with
+         | Hnil => fun x => x
+         | Hcons e es => fun f => rec _ es (f (exprD e))
+         end) ts xs u
     | eAbs f => fun x => exprD (f x)
     | eApp f x => exprD f (exprD x)
     | eTAbs f => fun x => exprD (f x)
     | eTApp f x => exprD f x
-  end
-  .
+  end.
 
-Example polyId {lF F Fe} : expr lF F Fe idType :=
-  eTAbs (fun t : type F kStar => eAbs (fun x : Fe (liftT t) => eVar x))
+Example polyId {lF F Ku Fe Fu} : expr lF F Ku Fu Fe idType :=
+  eTAbs (fun t : type F Ku kStar => eAbs (fun x : Fe (liftT t) => eVar x))
 .
 
-Example inst1 {lF F Fe} (t : type F kStar) : expr lF F Fe (liftT (smArr t t)) :=
+Example inst1 {lF F Ku Fe Fu} (t : type F Ku kStar) : expr lF F Ku Fe Fu (liftT (smArr t t)) :=
   eAbs (fun x => eApp (eTApp polyId t) (eVar x))
 .
 
-Example inst2 {lF F Fe} (t : type F kStar) : expr lF F Fe (liftT (smArr t t)) :=
+Example inst2 {lF F Ku Fu Fe} (t : type F Ku kStar) : expr lF F Ku Fu Fe (liftT (smArr t t)) :=
   eApp (eTApp polyId (smArr t t)) (eAbs (fun x => eVar x))
 .
 
-(* Local Variables: *)
-(* coq-prog-name: "/Users/matt/.opam/system/bin/coqtop" *)
-(* coq-load-path: nil *)
-(* End: *)
 
