theories/Poly/PolyP_unify.v
@@ -1,0 +1,207 @@
+Require Import ExtLib.Data.HList.
+Require Import MirrorCore.Poly.PolyPHOAS.
+
+(** UNIFICATION **)
+Section unify_type.
+
+(** With this representation, I lose the fact that Fu determines the list and the kind **)
+Let Fu : list kind -> kind -> Type := fun _ _ => nat.
+Let F : kind -> Type := fun _ => nat.
+
+Definition TSubst : Type :=
+  forall ks k, Fu ks k -> option (hlist (type Fu F) ks -> type Fu F k).
+
+
+Definition kind_eq_dec : forall a b : kind, {a = b} + {a <> b}.
+Proof. decide equality. Defined.
+
+Definition type_eq_dec : forall {k} (a b : type Fu F k), {a = b} + {a <> b}.
+Proof. Admitted.
+
+Definition TSubst_add {ks k} (u : Fu ks k) (val : hlist (type Fu F) ks -> type Fu F k) (s : TSubst) : TSubst :=
+  fun a b x =>
+    match PeanoNat.Nat.eq_dec u x with
+    | left _ =>
+      match List.list_eq_dec kind_eq_dec ks a
+            , kind_eq_dec k b
+      with
+      | left pf , left pf' =>
+        Some match pf in _ = X , pf' in _ = Y
+                   return hlist (type Fu F) X -> type Fu F Y
+             with
+             | eq_refl , eq_refl => val
+             end
+      | _ , _ => None
+      end
+    | right _ => s a b x
+    end.
+
+Fixpoint find_in_list {ks k} (x : type Fu F k) (ls : hlist (type Fu F) ks)
+: option (hlist (type Fu F) ks -> type Fu F k) :=
+  match ls in hlist _ ks
+        return option (hlist (type Fu F) ks -> type Fu F k)
+  with
+  | Hnil => None
+  | @Hcons _ _ k' _ l ls =>
+    match kind_eq_dec k' k with
+    | left pf =>
+      match @type_eq_dec k x match pf with
+                             | eq_refl => l
+                             end with
+      | left _ => Some (fun xs => match pf with
+                                  | eq_refl => hlist_hd xs
+                                  end)
+      | right _ =>
+        match find_in_list x ls with
+        | None => None
+        | Some v => Some (fun x => v (hlist_tl x))
+        end
+      end
+    | right _ =>
+      match find_in_list x ls with
+      | None => None
+      | Some v => Some (fun x => v (hlist_tl x))
+      end
+    end
+  end.
+
+Fixpoint pattern_type {ks k} (a : type Fu F k) (xs : hlist (type Fu F) ks)
+: option (hlist (type Fu F) ks -> type Fu F k).
+refine
+  match find_in_list a xs with
+  | Some x => Some x
+  | None =>
+    match a in type _ _ k
+          return option (hlist (type Fu F) ks -> type Fu F k)
+    with
+    | smUVar _ _ => None (* Bad *)
+    | smArr l r =>
+      match pattern_type _ _ l xs , pattern_type _ _ r xs with
+      | Some l' , Some r' => Some (fun a => smArr (l' a) (r' a))
+      | _ , _ => None
+      end
+    | smApp l r =>
+      match pattern_type _ _ l xs , pattern_type _ _ r xs with
+      | Some l' , Some r' => Some (fun a => smApp (l' a) (r' a))
+      | _ , _ => None
+      end
+    | smAbs t => None (** TODO **)
+    | smVar v => None
+    end
+  end.
+Defined.
+
+Variable unify' : forall {k} (f : nat) (a b : type Fu F k) (s : TSubst), option TSubst.
+
+
+Definition pattern_add {ks k} (u : Fu ks k) (xs : hlist (type Fu F) ks)
+           (e : type Fu F k) (s : TSubst) : option TSubst :=
+  match pattern_type e xs with
+  | None => None
+  | Some o' => Some (TSubst_add u o' s)
+  end.
+
+Fixpoint unify_type {k} (f : nat) (a b : type Fu F k) (s : TSubst) {struct a}
+: option TSubst.
+  refine (
+    match a in type _ _ k , b in type _ _ k' return k' = k -> option TSubst with
+    | smVar v , smVar v' => fun _ =>
+      if PeanoNat.Nat.eq_dec v v' then Some s else None
+    | smArr l r , smArr l' r' => fun _ =>
+      match unify_type _ f l l' s with
+      | Some s' => unify_type _ f r r' s
+      | _ => None
+      end
+    | @smApp _ _ k1 k2 l r , @smApp _ _ k1' k2' l' r' =>
+      fun pf =>
+        match kind_eq_dec k1' k1 with
+        | left pf' =>
+          match pf' in _ = X , pf in _ = Y
+                return (type Fu F (kArr X Y) -> TSubst -> option TSubst) ->
+                       (type Fu F X -> TSubst -> option TSubst) ->
+                       option TSubst
+          with
+          | eq_refl , eq_refl => fun rl rr =>
+                                   match rl l' s with
+                                   | Some s' => rr r' s'
+                                   | _ => None
+                                   end
+          end (fun x => unify_type _ f l x) (fun x => unify_type _ f r x)
+        | right _ => None
+        end
+    | @smAbs _ _ k1 k2 t , @smAbs _ _ k1' k2' t' => fun pf =>
+      match pf in _ = X
+            return match X with
+                   | kArr a b => (type Fu F b -> TSubst -> option TSubst) -> option TSubst
+                   | _ => unit
+                   end
+      with
+      | eq_refl => fun rec => rec (t' f) s
+      end (unify_type _ (S f) (t f))
+    | @smUVar _ _ ks k u xs , @smUVar _ _ ks' k' u' xs' => fun pf =>
+      match PeanoNat.Nat.eq_dec u u' with
+      | left pf' =>
+        match List.list_eq_dec kind_eq_dec ks' ks with
+        | left pf'' =>
+          (fix rec ls (xs : hlist (type Fu F) ls) (s : TSubst) : hlist (type Fu F) ls -> option TSubst :=
+             match xs in hlist _ ls
+                   return hlist (type Fu F) ls -> option TSubst
+             with
+             | Hnil => fun _ => Some s
+             | Hcons x xs => fun ys =>
+                               match unify' _ f x (hlist_hd ys) s with
+                               | None => None
+                               | Some s' => rec _ xs s' (hlist_tl ys)
+                               end
+             end)
+            ks xs s match pf'' with
+                    | eq_refl => xs'
+                    end
+        | _ => None
+        end
+      | _ =>
+        match s _ _ u , s _ _ u' with
+        | Some e , Some e' => unify' _ f (e xs) match pf with
+                                                | eq_refl => e' xs'
+                                                end s
+        | Some e , None => pattern_add u' xs' match eq_sym pf with
+                                              | eq_refl => e xs
+                                              end s
+        | None , Some e' => pattern_add u xs match pf with
+                                             | eq_refl => e' xs'
+                                             end s
+        | None , None =>
+          match pattern_add u xs match pf with
+                                 | eq_refl => smUVar u' xs'
+                                 end s with
+          | Some s => Some s
+          | None => pattern_add u' xs' match eq_sym pf with
+                                       | eq_refl => smUVar u xs
+                                       end s
+          end
+        end
+      end
+    | smUVar u xs , other => fun pf =>
+      match s _ _ u with
+      | None =>
+        pattern_add u xs match pf with
+                         | eq_refl => other
+                         end s
+      | Some e' => unify' _ f (e' xs) match pf with
+                                      | eq_refl => other
+                                      end s
+      end
+    | other , smUVar u xs => fun pf =>
+      match s _ _ u with
+      | None =>
+        pattern_add u xs match eq_sym pf with
+                         | eq_refl => other
+                         end s
+      | Some e' => unify' _ f match eq_sym pf with
+                              | eq_refl => other
+                              end (e' xs) s
+      end
+    | _ , _ => fun _ => None
+    end eq_refl).
+Defined.
+End unify_type.
